Moved registered to syntax.

src/AsyncFinish/Semantics.v
@@ -3,55 +3,6 @@ Require Import HJ.AsyncFinish.Rel.
 Require Import HJ.Vars.
 Require Import Coq.Lists.List.
 
-Inductive Registered (t:tid) (f:finish) : Prop :=
-  registered_def:
-    forall a,
-    Child (t, a) f ->
-    Registered t f.
-
-Lemma registered_cons:
-  forall t l p,
-  Registered t (Node l) ->
-  Registered t (Node (p::l)).
-Proof.
-  intros.
-  inversion H.
-  eauto using child_cons, registered_def.
-Qed.
-
-Lemma registered_eq:
-  forall t l a,
-  Registered t (Node ((t,a)::l)).
-Proof.
-  intros.
-  eauto using registered_def, child_eq.
-Qed.
-
-Lemma registered_absurd_nil:
-  forall t,
-  ~ Registered t (Node nil).
-Proof.
-  intros.
-  intuition.
-  inversion H.
-  apply child_absurd_nil in H0.
-  assumption.
-Qed.
-
-Lemma registered_inv_cons:
-  forall t t' a l,
-  Registered t (Node ((t', a) :: l)) ->
-  t = t' \/ Registered t (Node l).
-Proof.
-  intros.
-  inversion H.
-  apply child_inv_cons in H0.
-  destruct H0 as [Hx|?].
-  - inversion Hx; subst; clear Hx.
-    intuition.
-  - eauto using registered_def.
-Qed.
-
 Import Rel.
 Import Rel.Notations.
 Open Scope finish_scope.
